progress

theories/vir/examples/las.v
@@ -26,11 +26,13 @@ Section las_example.
 
   (* [a] is the register that will be analyzed for load after store
      [v] is the current register whose value is stored in the address at [a]. *)
+
   (* LATER: Can generalize the [v] values being stored (e.g. storing constants).
      FIXME: Generalize [v] to expressions *)
   (* TODO: Figure out if there is a normal form that can be enforced to make
    sure expressions refer to [local_id]s. *)
-  Fixpoint las_block {T} (b : code T) (a : raw_id) (v : option raw_id) :=
+  Fixpoint las_block {T} (b : code T) (a : raw_id) (v : option raw_id)
+    : code T :=
     match b with
     | nil => nil
     | x :: tl =>
@@ -60,7 +62,7 @@ Section las_example.
     end.
 
   (* Apply the [las] optimization over an open control flow graph. *)
-  Definition las_cfg {T} (o : ocfg T) a :=
+  Definition las_ocfg {T} (o : ocfg T) a : ocfg T :=
     List.map (fun x =>
       mk_block
         (blk_id x)
@@ -119,8 +121,11 @@ Section las_example.
   Definition promotable_block {T} (i : LLVMAst.block T) a : bool :=
     forallb (fun x => promotable_instr x a) (blk_code i).
 
+  Definition promotable_ocfg {T} (c : ocfg T) a :=
+    forallb (fun i => promotable_block i a) c.
+
   Definition promotable_cfg {T} (c : cfg T) a :=
-    forallb (fun i => promotable_block i a) (blks c).
+    promotable_ocfg (blks c) a.
 
   Definition find_promotable_alloca {T} (c : cfg T) :=
     (* LATER: Refactor this [instrs] comptuation? *)
@@ -132,14 +137,19 @@ Section las_example.
              end) instrs.
 
   (* Load-after-store optimization. *)
-  Definition las {T} (c : cfg T) :=
+  Definition las {T} (c : cfg T) : cfg T :=
     match find_promotable_alloca c with
       | Some (IId i, _) =>
           {| init := init c ;
-             blks := las_cfg (blks c) i ;
+             blks := las_ocfg (blks c) i ;
              args := args c |}
       | _ => c
     end.
+
+  Definition las_fun (f : definition dtyp (cfg dtyp)) : definition _ _ :=
+    {| df_prototype := df_prototype f;
+       df_args := df_args f;
+       df_instrs := las (df_instrs f) |}.
 
 End las_example.
 
@@ -155,13 +165,13 @@ Example code1 : code dtyp :=
   nil.
 
 Example block1 : LLVMAst.block dtyp :=
-    {|
-      blk_id    := Name "init_block";
-      blk_phis  := nil;
-      blk_code  := code1;
-      blk_term  := TERM_Ret (DTYPE_I 8%N, (EXP_Integer 8));
-      blk_comments := None
-    |}.
+  {|
+    blk_id    := Name "init_block";
+    blk_phis  := nil;
+    blk_code  := code1;
+    blk_term  := TERM_Ret (DTYPE_I 8%N, (EXP_Integer 8));
+    blk_comments := None
+  |}.
 
 Example ocfg1 : ocfg dtyp := block1 :: nil.
 
@@ -174,4 +184,95 @@ Compute (find_promotable_alloca cfg1).
 
 Compute (las cfg1).
 Compute (las_block code1 (Name "a")).
-(* TODO: Run it and Prove it *)
+
+(* ------------------------------------------------------------------- *)
+(* Specification of the Load-after-store optimization. *)
+
+Notation function := (definition dtyp (cfg dtyp)).
+
+(* TODO Get this definition from [contextual]. *)
+Axiom ctx_ref : function -> function -> Prop.
+Axiom fun_is_SSA : function -> Prop.
+Axiom ocfg_is_SSA : ocfg dtyp -> Prop.
+Axiom code_is_SSA : code dtyp -> Prop.
+
+From velliris Require Import vir.logical_relations.
+
+From velliris.program_logic Require Import program_logic.
+
+Section las_example_proof.
+
+Context `{vellirisGS Σ}.
+
+Definition ocfg_post_inv C i_t i_s A_t A_s : iPropI Σ :=
+  (∃ (args_t args_s : local_env),
+      ldomain_tgt i_t (list_to_set args_t.*1) ∗
+      ldomain_src i_s (list_to_set args_s.*1) ∗
+      stack_tgt i_t ∗ stack_src i_s ∗
+      frame_WF i_t i_s ∗
+      ([∗ list] '(l_t, v_t) ∈ args_t, [ l_t := v_t ]t i_t) ∗
+      ([∗ list] '(l_s, v_s) ∈ args_s, [ l_s := v_s ]s i_s) ∗
+  checkout C ∗
+  alloca_tgt i_t (list_to_set A_t : gset _) ∗
+  alloca_src i_s (list_to_set A_s : gset _) ∗
+  ⌜NoDup A_t⌝ ∗ ⌜NoDup A_s⌝)%I.
+
+(* TODO : make [logical relations] take in an invariant [I] *)
+
+Definition term_logrel ϒ_t ϒ_s I : iPropI Σ :=
+(⌜term_WF ϒ_t⌝ -∗
+ ⌜term_WF ϒ_s⌝ -∗
+    I -∗
+    exp_conv (denote_terminator ϒ_t) ⪯
+    exp_conv (denote_terminator ϒ_s)
+    [{ (r_t, r_s), I ∗
+                    match r_t, r_s with
+                    | inl b_t, inl b_s => ⌜b_t = b_s⌝
+                    | inr v_t, inr v_s => uval_rel v_t v_s
+                    | _, _ => False
+                    end}])%I.
+
+(* Factor out for use in general optimizations *)
+Lemma simulation_ocfg (a : raw_id) Φ I cfg_t cfg_s i_t i_s A_t A_s b1 b2 :
+  ⊢ (code_inv ∅ i_t i_s A_t A_s -∗ I) -∗
+    (I -∗ ∃ A_t' A_s',
+            ocfg_post_inv ∅ i_t i_s A_t' A_s') -∗
+    (* Related terminators *)
+    (∀ (i : nat) b_t b_s,
+      ⌜cfg_t !! i = Some b_t⌝ -∗
+      ⌜cfg_s !! i = Some b_s⌝ -∗
+      term_logrel (blk_term b_t) (blk_term b_s) I) -∗
+    (* Related instructions *)
+    (∀ (i : nat) b_t b_s,
+      ⌜cfg_t !! i = Some b_t⌝ -∗
+      ⌜cfg_s !! i = Some b_s⌝ -∗
+      I -∗
+      instr_conv (denote_code (blk_code b_t)) ⪯
+      instr_conv (denote_code (blk_code b_s))
+      [{ (r_t, r_s), I ∗ Φ r_t r_s }]) -∗
+   (* TODO: state [phi_logrel] related for a weakened [phi_logrel] *)
+   (* Weaken the postcondition for [ocfg_logrel] *)
+    ocfg_logrel cfg_t cfg_s ∅ A_t A_s b1 b2.
+Proof. Admitted.
+
+Lemma las_simulation_ocfg
+  (f : ocfg dtyp) a A_t A_s b1 b2 :
+  ocfg_is_SSA f ->
+  promotable_ocfg f a ->
+  ⊢ ocfg_logrel (las_ocfg f a) f ∅ A_t A_s b1 b2.
+Proof.
+Admitted.
+
+Lemma las_simulation (f : function) :
+  fun_is_SSA f ->
+  ⊢ fun_logrel (las_fun f) f ∅.
+Proof. Admitted.
+
+Theorem las_correct (c : function) :
+  fun_is_SSA c ->
+  ctx_ref (las_fun c) c.
+Proof. Admitted.
+
+(* TODO: Prove it *)
+
+End las_example_proof.
