theories/vir/spec.v
@@ -23,9 +23,24 @@ Notation "# l" := (DVALUE_Addr (to_addr l)) (at level 30).
 
 Notation "d  ̂" := (dvalue_to_uvalue d) (at level 40).
 
+#[global] Instance attr_eq_dec: EqDecision fn_attr.
+Proof. solve_decision. Defined.
+
+Definition HasAttr : fn_attr -> list fn_attr -> bool :=
+  fun attr l => 
+    match l with
+    | nil => false
+    | l => 
+      foldl (fun p b => 
+        p || (Coqlib.proj_sumbool (decide (b = attr)))) false l
+    end.
+
+Definition HaveAttr : fn_attr -> list fn_attr -> list fn_attr -> bool :=
+  fun attr l l' => HasAttr attr l && HasAttr attr l'.
+
 (** *Attribute specifications *)
 Section spec.
-  Context Σ `{!sheapGS Σ, !checkedoutGS Σ, !heapbijGS Σ}.
+  Context Σ `{!vellirisGS Σ}.
 
   Definition frame_WF {A} (i_t i_s : list A) : iPropI Σ :=
     ((⌜length i_s > 0 -> length i_t > 0⌝)%Z)%I.
@@ -34,22 +49,135 @@ Section spec.
     let h := (vir_heap state.(vmem)) in
     ⌜h !! a = v⌝.
 
+  Variant attr_case : Type :=
+  | ARG_READ
+  | WRITEONLY
+  | NOFREE
+  | ARGMONLY
+  | READONLY
+  | INACC_OR_ARGMONLY
+  | OTHER.
+
+  (** *Specification of memory-related function attributes
+
+      Invariants about the checked-out set that holds before and after a call. *)
+  (* For now, we only express invariants for specific attribute lists (instead of
+     allowing for an arbitrary number of attribute combinations and disallowing
+     certain combinations). *)
+  Equations attribute_interp :
+    ∀ {X Y : Type}, ExternalCallE X → ExternalCallE Y → gmap (loc * loc) Qp -> Prop :=
+    attribute_interp
+      (ExternalCall a f args_t attr_t)
+      (ExternalCall a0 f0 args_s attr_s) C :=
+       let attr_t := remove_tag attr_t in
+       let attr_s := remove_tag attr_s in
+       let have := fun attr => HaveAttr attr attr_t attr_s in
+       ∃ (c : attr_case),
+         match c with
+         | ARG_READ => have FNATTR_Argmemonly && have FNATTR_Readonly /\
+              (∀ l_t l_s n,
+                  nth_error (zip args_t args_s) n =
+                    Some (UVALUE_Addr l_t, UVALUE_Addr l_s) ->
+                      ∃ q, C !! (l_t.1, l_s.1) = Some q ∧ Qp.lt q 1)
+         | WRITEONLY => have FNATTR_Writeonly /\ C = ∅
+         | NOFREE => have FNATTR_Nofree /\ C = ∅
+         | ARGMONLY => have FNATTR_Argmemonly /\ not (have FNATTR_Readonly) /\
+                      (∀ l_t l_s n,
+                        nth_error (zip args_t args_s) n =
+                          Some (UVALUE_Addr l_t, UVALUE_Addr l_s) ->
+                        C !! (l_t.1, l_s.1) = None)
+         | READONLY => have FNATTR_Readonly /\ not (have FNATTR_Argmemonly) /\
+                        (∀ (l_t l_s : loc) q, C !! (l_t, l_s) = Some q -> Qp.lt q 1)
+         | INACC_OR_ARGMONLY => have FNATTR_Inaccessiblemem_or_argmemonly /\
+                      (∀ l_t l_s n,
+                        nth_error (zip args_t args_s) n =
+                          Some (UVALUE_Addr l_t, UVALUE_Addr l_s) ->
+                        C !! (l_t.1, l_s.1) = None) /\
+                      (∀ (l_t l_s : Z * Z),
+                          (l_t.1, l_s.1) ∈ dom C ->
+                          (UVALUE_Addr l_t, UVALUE_Addr l_s) ∉ (zip args_t args_s) ->
+                          C !! (l_t.1, l_s.1) = Some 1%Qp)
+         | OTHER =>
+             not (have FNATTR_Argmemonly) /\
+             not (have FNATTR_Readonly) /\
+             not (have FNATTR_Writeonly) /\
+             not (have FNATTR_Nofree) /\
+             not (have FNATTR_Inaccessiblemem_or_argmemonly) /\
+                  let ev_t := ExternalCall a f args_t attr_t in
+                  let ev_s := ExternalCall a0 f0 args_s attr_s in
+                   ev_t ~= ev_s /\ C = ∅
+         end.
+
   Equations vir_call_ev {X Y} :
     language.CallE (call_events vir_lang) X →
     language.CallE (call_events vir_lang) Y →
-    (list frame_names * list frame_names)%type -> iPropI Σ :=
-    vir_call_ev (ExternalCall t f args attr) (ExternalCall t0 f0 args0 attr0) (i_t, i_s) :=
+    (gmap (loc * loc) Qp * list frame_names * list frame_names)%type -> iPropI Σ :=
+    vir_call_ev (ExternalCall t f args attr) (ExternalCall t0 f0 args0 attr0) (C, i_t, i_s) :=
       (dval_rel f f0 ∗
         ⌜t = t0⌝ ∗ ⌜attr = attr0⌝ ∗ ([∗ list] x;y ∈ args; args0, uval_rel x y) ∗
-        checkout ∅ ∗ frame_WF i_t i_s ∗ stack_tgt i_t ∗ stack_src i_s)%I.
+        checkout C ∗ frame_WF i_t i_s ∗ stack_tgt i_t ∗ stack_src i_s ∗
+        ⌜attribute_interp (ExternalCall t f args attr) (ExternalCall t0 f0 args0 attr0) C⌝)%I.
 
   Equations vir_call_ans {X Y : Type} :
     language.CallE (call_events vir_lang) X → X ->
     language.CallE (call_events vir_lang) Y → Y ->
-    (list frame_names * list frame_names) -> iPropI Σ :=
+    (gmap (loc * loc) Qp * list frame_names * list frame_names) -> iPropI Σ :=
       vir_call_ans (ExternalCall t f args attr) v_t
-                  (ExternalCall t0 f0 args0 attr0) v_s (i_t, i_s) :=
-        (checkout ∅ ∗ stack_tgt i_t ∗ stack_src i_s ∗ uval_rel v_t v_s)%I.
+                  (ExternalCall t0 f0 args0 attr0) v_s (C, i_t, i_s) :=
+        (checkout C ∗ stack_tgt i_t ∗ stack_src i_s ∗ uval_rel v_t v_s)%I.
+
+  (* Readonly :
+      initial and final states are identical. *)
+  Equations readonly_ans_spec {R1 R2}
+    (ev_t : CallEvents vir_lang R1) (v_t : R1) (ev_s : CallEvents vir_lang R2) (v_s : R2) : Prop :=
+    readonly_ans_spec
+      (StateEff (call_events vir_lang) (s, ExternalCall t f args attr)) v_t
+      (StateEff (call_events vir_lang) (s0, ExternalCall t0 f0 args0 attr0)) v_s :=
+    (v_t.1 = s /\ v_s.1 = s0).
+
+  (* ArgMemOnly :
+      All addr arguments have related values stored in the heap *)
+  Equations argmemonly_ev_spec {R1 R2}
+    (ev_t : CallEvents vir_lang R1) (ev_s : CallEvents vir_lang R2) : Prop :=
+    argmemonly_ev_spec
+      (StateEff (call_events vir_lang) (s, ExternalCall t f args attr))
+      (StateEff (call_events vir_lang) (s0, ExternalCall t0 f0 args0 attr0)) :=
+    (forall a v, UVALUE_Addr (a, 0)%Z ∈ args -> vir_heap (vmem s) !! a = Some v ->
+            exists a0 v0, UVALUE_Addr (a0, 0)%Z ∈ args0 /\ vir_heap (vmem s0) !! a0 = Some v0 /\ v = v0) /\
+    (forall a v, UVALUE_Addr (a, 0) ∈ args0 -> vir_heap (vmem s0) !! a = Some v ->
+            exists a0 v0, UVALUE_Addr (a0, 0)%Z ∈ args /\ vir_heap (vmem s) !! a0 = Some v0 /\ v = v0).
+
+  (* Every piece of state that is not part of the arguments is unchanged. *)
+  Equations argmemonly_ans_spec {R1 R2}
+    (ev_t : CallEvents vir_lang R1) (v_t : R1) (ev_s : CallEvents vir_lang R2) (v_s : R2) : Prop :=
+    argmemonly_ans_spec
+      (StateEff (call_events vir_lang) (s, ExternalCall t f args attr)) v_t
+      (StateEff (call_events vir_lang) (s0, ExternalCall t0 f0 args0 attr0)) v_s :=
+    ((∀ a v, vir_heap (vmem v_t.1) !! a = Some v ->
+                UVALUE_Addr (a, 0) ∉ args ->
+                vir_heap (vmem s) !! a = Some v) /\
+          (∀ a v, vir_heap (vmem v_s.1) !! a = Some v ->
+                  UVALUE_Addr (a, 0) ∉ args ->
+                  vir_heap (vmem s0) !! a = Some v)).
+
+  (* Specification for [nofree] and [writeonly] *)
+  Equations no_free_ans_spec {R1 R2}
+    (ev_t : CallEvents vir_lang R1) (v_t : R1) (ev_s : CallEvents vir_lang R2) (v_s : R2) : Prop :=
+    no_free_ans_spec
+      (StateEff (call_events vir_lang) (s, ExternalCall t f args attr)) v_t
+      (StateEff (call_events vir_lang) (s0, ExternalCall t0 f0 args0 attr0)) v_s :=
+      (forall a v, vir_heap (vmem s) !! a = Some v ->
+             exists v', vir_heap (vmem v_t.1) !! a = Some v') /\
+      (forall a v, vir_heap (vmem s0) !! a = Some v ->
+             exists v', vir_heap (vmem v_s.1) !! a = Some v').
+
+  Definition vir_E_ans : ∀ X Y : Type, E vir_lang X → X → E vir_lang Y → Y → Prop :=
+    λ (X Y : Type) (X0 : E vir_lang X) (X1 : X) (X2 : E vir_lang Y) (X3 : Y),
+      (X1 ~= X3 ∧ X0 ~= X2).
+
+  Definition vir_call_ev_ : ∀ X Y : Type, CallEvents vir_lang X → CallEvents vir_lang Y → Prop :=
+    λ (X Y : Type) (e1 : CallEvents vir_lang X) (e2 : CallEvents vir_lang Y),
+    argmemonly_ev_spec e1 e2.
 
   Definition vir_E_ev : ∀ X Y : Type, E vir_lang X → E vir_lang Y → Prop :=
     λ (X Y : Type) (X0 : E vir_lang X) (X2 : E vir_lang Y), X0 ~= X2.
@@ -86,20 +214,20 @@ Section spec.
       call_ev := @vir_call_ev;
       call_ans := @vir_call_ans;
       arg_val_rel :=
-        (λ '(u0, l0) '(u, l) '(i_t, i_s),
+        (λ '(u0, l0) '(u, l) '(C, i_t, i_s),
           frame_WF i_t i_s ∗
-          checkout ∅ ∗ stack_tgt i_t ∗ stack_src i_s ∗
+          checkout C ∗ stack_tgt i_t ∗ stack_src i_s ∗
             dval_rel u0 u ∗ [∗ list] x;y ∈ l0; l, uval_rel x y)%I;
       res_val_rel :=
-        (λ u v '(i_t, i_s),
-          checkout ∅ ∗ stack_tgt i_t ∗ stack_src i_s ∗
+        (λ u v '(C, i_t, i_s),
+          checkout C ∗ stack_tgt i_t ∗ stack_src i_s ∗
            uval_rel u v)%I ; |}.
 
 End spec.
 
 Arguments frame_WF {_ _}.
 
-#[global] Instance SimE_vir_iProp {Σ} `{!sheapGS Σ, !checkedoutGS Σ, !heapbijGS Σ}:
+#[global] Instance SimE_vir_iProp {Σ} `{!vellirisGS Σ}:
   SimE (iPropI Σ) vir_lang := sim_expr_stutter (η := vir_handler).
 
 Arguments sim_coind_ub {_ _ _ _ _} [_] {_ _ _ _ _}.
@@ -109,7 +237,7 @@ From ITree Require Import Events.StateFacts.
 
 Section vir_sim_properties.
 
-  Context {Σ} `{!sheapGS Σ, !checkedoutGS Σ, !heapbijGS Σ}.
+  Context {Σ} `{!vellirisGS Σ}.
 
   Lemma sim_expr_exception {R} (e : _ R) s0 Φ:
     ⊢ e ⪯ trigger (Exception.Throw (print_msg s0)) [{ Φ }].
@@ -158,7 +286,7 @@ Notation "et '⪯' es [[ Φ ]]" :=
 
 Section conv_properties.
 
-  Context {Σ} `{!sheapGS Σ, !checkedoutGS Σ, !heapbijGS Σ}.
+  Context {Σ} `{!vellirisGS Σ}.
 
   Notation st_expr_rel' R1 R2 :=
     (@st_exprO' vir_lang R1 -d> @st_exprO' vir_lang R2 -d> iPropI Σ).
